Add more work towards preservation theorem with doubly nameless

src/Env.v
@@ -14,9 +14,11 @@ Module Env (P : PAT).
   Inductive binding : Type :=
   | BindTname : binding
   | BindCon   : data -> type -> tname -> binding
-  | BindTvar  : option kind -> binding
-  | BindVar   : option type -> binding
+  | BindTvar  : kind -> binding
+  | BindVar   : type -> binding
   | BindMatch : match_assum -> binding
+  | SkipTvar  : binding
+  | SkipVar   : binding
   .
 
   Definition env : Type := list binding.
@@ -27,11 +29,18 @@ Module Env (P : PAT).
   Definition is_con (b : binding) : Prop := match b with BindCon _ _ _ => True | _ => False end.
   Definition cons   (Gamma : env) : env := filter is_con Gamma.
 
-  Definition is_tvar (b : binding) : Prop := match b with BindTvar _ => True | _ => False end.
+  Definition is_tvar (b : binding) : Prop :=
+    match b with BindTvar _ => True | SkipTvar => True | _ => False end.
+  #[export]
+  Hint Unfold is_tvar : mcore.
   Definition tvars   (Gamma : env) : env := filter is_tvar Gamma.
 
-  Definition is_var (b : binding) : Prop := match b with BindVar _ => True | _ => False end.
+  Definition is_var (b : binding) : Prop :=
+    match b with BindVar _ => True | SkipVar => True | _ => False end.
+  #[export]
+  Hint Unfold is_var : mcore.
   Definition vars   (Gamma : env) : env := filter is_var Gamma.
+
 
   Definition is_match (b : binding) : Prop := match b with BindMatch _ => True | _ => False end.
   Definition matches  (Gamma : env) : env := filter is_match Gamma.
@@ -42,14 +51,35 @@ Module Env (P : PAT).
   Definition con_in (K : con) (d : data) (ty : type) (T : tname) (Gamma : env) : Prop :=
     Nth K Gamma (BindCon d ty T).
 
-  Definition tvar_in (tv : tvar) (k : option kind) (Gamma : env) : Prop :=
+  Definition tvar_in (tv : tvar) (k : kind) (Gamma : env) : Prop :=
     Nth tv Gamma (BindTvar k).
 
-  Definition var_in (v : var) (ty : option type) (Gamma : env) : Prop :=
+  Definition var_in (v : var) (ty : type) (Gamma : env) : Prop :=
     Nth v Gamma (BindVar ty).
 
   Definition empty_env : env := [ ].
 
+
+  Create HintDb rew_env.
+
+  Tactic Notation "rew_env" :=
+    autorewrite with rew_env.
+  Tactic Notation "rew_env" "~" :=
+    rew_env; auto_tilde.
+  Tactic Notation "rew_env" "*" :=
+    rew_env; auto_star.
+  Tactic Notation "rew_env" "in" "*" :=
+    autorewrite_in_star_patch ltac:(fun tt => autorewrite with rew_env).
+  Tactic Notation "rew_env" "~" "in" "*" :=
+    rew_env in *; auto_tilde.
+  Tactic Notation "rew_env" "*" "in" "*" :=
+    rew_env in *; auto_star.
+  Tactic Notation "rew_env" "in" hyp(H) :=
+    autorewrite with rew_env in H.
+  Tactic Notation "rew_env" "~" "in" hyp(H) :=
+    rew_env in H; auto_tilde.
+  Tactic Notation "rew_env" "*" "in" hyp(H) :=
+    rew_env in H; auto_star.
 
 
   Lemma vars_app : forall G1 G2, vars (G1 ++ G2) = vars G1 ++ vars G2.
@@ -59,11 +89,12 @@ Module Env (P : PAT).
       vars (b :: Gamma) =
         match b with
         | BindVar _ => b :: vars Gamma
+        | SkipVar   => b :: vars Gamma
         | _         => vars Gamma
         end.
-  Proof. intros ; destruct b ; unfold vars ; rew_listx ; rew_mcore~. Qed.
+  Proof. intros ; destruct b ; unfolds ; unfolds is_var ; rew_listx ; case_if*. Qed.
 
   #[export]
-  Hint Rewrite vars_app vars_cons : rew_mcore.
+  Hint Rewrite vars_app vars_cons : rew_env.
 
 End Env.
