src/Soundness.v
@@ -1,5 +1,8 @@
 From MCore Require Import Syntax Typing SmallStep Tactics.
-From TLC Require Import LibString LibNat LibList LibOrder.
+From TLC Require Import LibString LibList LibNat.
+Import LibListNotation.
+
+Open Scope nat_scope.
 
 Module Soundness (P : PAT).
   Module S := SmallStep P.
@@ -29,36 +32,114 @@ Module Soundness (P : PAT).
         inverts* Hval. inverts ttype. }
     Qed.
 
-    Lemma defreshen_freshen : forall t x, tm_defreshen (tm_freshen t x) x = t.
-    Proof.
-      intros. induction t ; simpls ; fequals*.
-      { Case "TmFVar". case_if as Hge ; simpls.
-        { case_if as Hgt ; rew_nat*.
-          cuts* Hgt' : (S v > x). rewrite gt_as_slt. rewrite lt_peano. rewrite* Nat.lt_succ_r. }
-        { case_if*. false. apply Hge. apply gt_to_ge. auto. } }
-    Qed.
+    Lemma tm_defreshen_freshen : forall t x, tm_defreshen (tm_freshen t x) x = t.
+    Proof. intros ; induction t ; simple_math ; simpls ; fequals*. Qed.
 
-    Lemma freshen_fresh : forall t x, var_fresh x (tm_freshen t x).
-    Proof. intros. unfold var_fresh. rewrite* defreshen_freshen. Qed.
+    Lemma ty_defreshen_freshen : forall t x, ty_defreshen (ty_freshen t x) x = t.
+    Proof. intros ; induction t ; simple_math ; simpls ; fequals*. Qed.
+
+    Lemma tm_freshen_fresh : forall t x, var_fresh x (tm_freshen t x).
+    Proof. intros ; unfold var_fresh ; rewrite* tm_defreshen_freshen. Qed.
+
+    Lemma ty_freshen_fresh : forall t x, tvar_fresh x (ty_freshen t x).
+    Proof. intros ; unfold tvar_fresh ; rewrite* ty_defreshen_freshen. Qed.
 
     Lemma var_not_fresh : forall x, ~(var_fresh x (TmFVar x)).
     Proof.
-      intros x Heq. unfolds var_fresh. simpls.
-      case_if as Hgt.
-      - false. apply* Hgt.
-      - simpls. case_if as Hge.
-        * inverts Heq as contra. applys* Nat.neq_succ_diag_r.
-        * false. apply* Hge. apply ge_refl.
+      introv Heq. unfolds var_fresh. simple_math.
+      inverts Heq ; nat_math.
     Qed.
 
-    Lemma subst_fresh : forall t x u, var_fresh x t -> tm_subst t x u = t.
+    Lemma tvar_not_fresh : forall x, ~(tvar_fresh x (TyFVar x)).
     Proof.
-      introv Hfresh. unfolds tm_subst.
-      induction* t ; fequals ; inverts Hfresh as Hfresh1 Hfresh2 ;
-        try rewrite* Hfresh1 ; try rewrite* Hfresh2.
-      { Case "TmFVar". assert (Hneq : v <> x). intros Heq. subst.
-        lets* Hnfresh : var_not_fresh. case_if*. }
+      introv Heq. unfolds tvar_fresh. simple_math.
+      inverts Heq ; nat_math.
     Qed.
+
+    Lemma var_neq_fresh : forall x y, x <> y -> var_fresh x (TmFVar y).
+    Proof.
+      introv Hneq. unfolds. simple_math.
+      forwards [ k [ Heq Hle ] ] : Nat.lt_exists_pred x y ; subst ; rew_nat*.
+    Qed.
+
+    Lemma tm_subst_fresh : forall t x u, var_fresh x t -> tm_subst t x u = t.
+    Proof.
+      introv Hfresh. unfolds.
+      induction* t ; fequals ; try (injection Hfresh ; auto_star).
+      { Case "TmFVar". cases_if*. lets* ? : var_not_fresh v. }
+    Qed.
+
+    Lemma tm_freshen_freshen :
+      forall t x y,
+        x <= y ->
+        tm_freshen (tm_freshen t y) x = tm_freshen (tm_freshen t x) (S y).
+    Proof. introv Hle ; induction t ; simple_math ; try solve [ simpls ; fequals* ]. Qed.
+
+    Lemma tm_ty_freshen_comm :
+      forall t x y,
+        tm_ty_freshen (tm_freshen t x) y = tm_freshen (tm_ty_freshen t y) x.
+    Proof. intros ; induction t ; simple_math ; simpls ; fequals*. Qed.
+
+    Lemma tm_freshen_subst :
+      forall t x y u,
+        x <= y ->
+        tm_freshen (tm_subst t y u) x =
+          tm_subst (tm_freshen t x) (S y) (tm_freshen u x).
+    Proof. introv Hge ; induction t ; simple_math ; simpls ; fequals*. Qed.
+
+    Lemma tm_freshen_bsubst : forall t y z u,
+        tm_freshen (tm_bsubst t y u) z =
+          tm_bsubst (tm_freshen t z) y (tm_freshen u z).
+    Proof. induction t ; intros ; simple_math ; simpls ; fequals*. Qed.
+
+    Lemma ty_freshen_bsubst : forall t y z u,
+        ty_freshen (ty_bsubst t y u) z =
+          ty_bsubst (ty_freshen t z) y (ty_freshen u z).
+    Proof. induction t ; intros ; simple_math ; simpls ; fequals*. Qed.
+
+    Lemma tm_ty_freshen_bsubst : forall t y z u,
+        tm_freshen (tm_ty_bsubst t y u) z =
+          tm_ty_bsubst (tm_freshen t z) y u.
+    Proof. induction t ; intros ; simple_math ; simpls ; fequals*. Qed.
+
+    Lemma tm_freshen_lc : forall t x, tm_lc t -> tm_lc (tm_freshen t x).
+    Proof.
+      introv Hlc. unfold tm_freshen.
+      gen x.
+      induction Hlc ; intros ; simpls*.
+      { Case "TmFVar". case_if*. }
+      { Case "TmLam". constructor*. unfolds tm_open.
+        rewrite tm_freshen_freshen ; try nat_math.
+        assert (Hfv : TmFVar 0 = tm_freshen (TmFVar 0) (S x)) by simple_math.
+        rewrite Hfv. rewrite* <- tm_freshen_bsubst. }
+      { Case "TmTyLam". constructor*. unfolds tm_ty_open.
+        rewrite tm_ty_freshen_comm. rewrite* <- tm_ty_freshen_bsubst. }
+    Qed.
+
+    Lemma ty_freshen_lc : forall ty x, ty_lc ty -> ty_lc (ty_freshen ty x).
+    Admitted.
+
+    Lemma ty_defreshen_lc : forall ty x, ty_lc ty -> ty_lc (ty_defreshen ty x).
+    Admitted.
+    (* Proof. *)
+    (*   introv Hlc. unfold tm_freshen. *)
+    (*   gen n. *)
+    (*   induction Hlc ; intros ; simpls*. *)
+    (*   { Case "TmFVar". case_if*. } *)
+    (*   { Case "TmLam". constructor*. unfolds tm_open. *)
+    (*     rewrite tm_freshen_freshen ; try nat_math. *)
+    (*     assert (Hfv : TmFVar 0 = tm_freshen (TmFVar 0) (S n)) by simple_math. *)
+    (*     rewrite Hfv. rewrite* <- tm_freshen_bsubst. } *)
+    (*   { Case "TmTyLam". constructor*. unfolds tm_ty_open. *)
+    (*     rewrite tm_ty_freshen_comm. rewrite* <- tm_ty_freshen_bsubst. } *)
+    (* Qed. *)
+
+    Lemma ty_lc_subst :
+      forall ty1 ty2 x,
+        ty_lc ty1 ->
+        ty_lc ty2 ->
+        ty_lc (ty_subst ty1 x ty2).
+    Admitted.
 
     (* TODO: can freshen be separated out from these lemmas into separate ones? *)
     Lemma ty_bsubst_neq : forall ty x y U1 U2,
@@ -90,7 +171,7 @@ Module Soundness (P : PAT).
       induction* t ; intros ; inverts Heq ; simpls ; fequals*.
     Qed.
 
-    Lemma lc_bsubst : forall t y u, tm_lc t -> tm_bsubst t y u = t.
+    Lemma tm_bsubst_lc : forall t y u, tm_lc t -> tm_bsubst t y u = t.
     Proof.
       introv Hlc. gen y.
       induction Hlc ; intros ; simpls ; fequals*.
@@ -98,72 +179,95 @@ Module Soundness (P : PAT).
       { Case "TmTyLam". rewrite tm_ty_bsubst_neq with (x := 0) (ty := TyFVar 0) ; auto. }
     Qed.
 
-    Lemma subst_bsubst_distr :
+    Lemma tm_subst_bsubst_distr :
       forall x y t u1 u2,
         tm_lc u1 ->
         tm_subst (tm_bsubst t y u2) x u1 =
           tm_bsubst (tm_subst t x u1) y (tm_subst u2 x u1).
     Proof.
-      introv Hlc. unfolds tm_bsubst. gen y.
-      induction t ; intros ; simpls*; fequals*.
-      { case_if*. }
-      { case_if*. rewrite* lc_bsubst. }
+      introv Hlc. unfolds. gen y.
+      induction t ; intros ; simpls ; fequals*.
+      { Case "TmBVar". case_if*. }
+      { Case "TmFVar". case_if*. rewrite* tm_bsubst_lc. }
     Qed.
 
-    (* Does this really need lc? *)
-    Lemma subst_intro :
+    Lemma tm_subst_intro :
       forall x y t u,
         var_fresh x t ->
-        tm_lc u ->
         tm_bsubst t y u = tm_subst (tm_bsubst t y (TmFVar x)) x u.
     Proof.
-      introv Hfresh Hlc. unfolds. rewrite* subst_bsubst_distr.
-      simpls. case_if. rewrite* subst_fresh.
+      introv Hfresh. unfolds. gen y.
+      induction t ; intros ; simpls ; fequals
+      ; try (injection Hfresh ; auto_star).
+      { Case "TmBVar". simple_math. }
+      { Case "TmFVar". cases_if*. lets* ? : var_not_fresh v. }
+    Qed.
+
+    Lemma ty_subst_intro :
+      forall x y ty u,
+        tvar_fresh x ty ->
+        ty_bsubst ty y u = ty_subst (ty_bsubst ty y (TyFVar x)) x u.
+    Proof.
+      introv Hfresh. unfolds. gen y.
+      induction ty ; intros ; simpls ; fequals
+      ; try (injection Hfresh ; auto_star).
+      { Case "TmBVar". simple_math. }
+      { Case "TmFVar". cases_if*. lets* ? : tvar_not_fresh t. }
+    Qed.
+
+    Lemma tm_subst_open :
+      forall t u,
+        tm_bsubst t 0 u = tm_defreshen (tm_subst (tm_open t) 0 (tm_freshen u 0)) 0.
+    Proof.
+      intros.
+      rewrite <- tm_defreshen_freshen with (x := 0) (t := tm_bsubst t 0 u).
+      rewrite tm_freshen_bsubst. rewrite* (@tm_subst_intro 0). apply tm_freshen_fresh.
+    Qed.
+
+    Lemma ty_subst_open :
+      forall ty u,
+        ty_bsubst ty 0 u = ty_defreshen (ty_subst (ty_open ty) 0 (ty_freshen u 0)) 0.
+    Proof.
+      intros.
+      rewrite <- ty_defreshen_freshen with (x := 0) (t := ty_bsubst ty 0 u).
+      rewrite ty_freshen_bsubst. rewrite* (@ty_subst_intro 0). apply ty_freshen_fresh.
+    Qed.
+
+    Lemma tm_bsubst_subst_comm :
+      forall t x y z u,
+        x <> z ->
+        tm_lc u ->
+        tm_bsubst (tm_subst t x u) y (TmFVar z) =
+          tm_subst (tm_bsubst t y (TmFVar z)) x u.
+    Proof.
+      introv Hneq Hlc. symmetry.
+      applys_eq* tm_subst_bsubst_distr. fequals.
+      rewrite* tm_subst_fresh. apply* var_neq_fresh.
     Qed.
 
     Lemma tm_open_subst_comm :
       forall t x u,
         tm_lc u ->
         tm_open (tm_subst t x u) = tm_subst (tm_open t) (S x) (tm_freshen u 0).
-    Proof. Admitted.
+    Proof.
+      introv Hlc. unfolds. rewrite tm_freshen_subst. applys* tm_bsubst_subst_comm.
+      apply* tm_freshen_lc. nat_math.
+    Qed.
 
     Lemma tm_ty_open_subst_comm :
-      forall t n t',
-        tm_lc t' ->
-        tm_ty_open (tm_subst t n t') = tm_subst (tm_ty_open t) n (tm_ty_freshen t' 0).
+      forall t x u,
+        tm_lc u ->
+        tm_ty_open (tm_subst t x u) = tm_subst (tm_ty_open t) x (tm_ty_freshen u 0).
     Proof. Admitted.
 
     Lemma tm_open_defreshen_comm :
-      forall t n,
-        tm_open (tm_defreshen t n) = tm_defreshen (tm_open t) (S n).
+      forall t x,
+        tm_open (tm_defreshen t x) = tm_defreshen (tm_open t) (S x).
     Proof. Admitted.
 
     Lemma tm_ty_open_defreshen_comm :
-      forall t n,
-        tm_ty_open (tm_defreshen t n) = tm_defreshen (tm_ty_open t) n.
-    Proof. Admitted.
-
-    Lemma bsubst_subst :
-      forall t t',
-        tm_freshen (tm_bsubst t 0 t') 0 =
-          tm_subst (tm_open t) 0 (tm_freshen t' 0).
-    Proof.
-      intros.
-      induction t.
-      { Case "TmBVar". unfold tm_bsubst. unfold tm_open. unfold tm_freshen. unfold tm_bsubst.
-        unfold tm_subst. unfold tm_defreshen. destruct v. case_if*. case_if*. unfold
-      }
-
-    Lemma tm_freshen_preservation :
-      forall Gamma t ty ty',
-        ok_term Gamma t ty ->
-        ok_term (BindVar ty' :: Gamma) (tm_freshen t 0) ty.
-    Proof. Admitted.
-
-    Lemma tm_ty_freshen_preservation :
-      forall Gamma t ty k',
-        ok_term Gamma t ty ->
-        ok_term (BindTvar k' :: Gamma) (tm_ty_freshen t 0) ty.
+      forall t x,
+        tm_ty_open (tm_defreshen t x) = tm_defreshen (tm_ty_open t) x.
     Proof. Admitted.
 
     Lemma ok_type_lct :
@@ -172,21 +276,24 @@ Module Soundness (P : PAT).
         ty_lc ty.
     Proof. introv tykind. induction* tykind. Qed.
 
+    Lemma ok_env_type :
+      forall G1 G2 ty,
+        ok_env (G1 ++ BindVar ty :: G2) ->
+        ok_type G2 ty KiType.
+    Proof. introv Henv ; induction* G1 ; inverts* Henv. Qed.
+
     Lemma ok_env_lct :
-      forall Gamma ty x,
+      forall Gamma x ty,
         ok_env Gamma ->
-        var_in x (Some ty) (vars Gamma) ->
+        var_in x ty (vars Gamma) ->
         ty_lc ty.
     Proof.
-      introv Henv. gen x.
-      induction* Gamma ; intros ; with_hyp (var_in _ _ _) as Hvar. inverts Hvar.
-      destruct a; rew_mcore in *; inverts* Henv ; unfold var_in in Hvar.
-      { lets [ (Heq0 & Heqty) | (m & Heqm & in_Gamma) ] : Nth_cons_inv Hvar ; subst.
-        { inverts Heqty. apply* ok_type_lct. }
-        { apply* IHGamma. } }
-      { lets [ (Heq0 & Heqty) | (m & Heqm & in_Gamma) ] : Nth_cons_inv Hvar ; subst.
-        { inverts Heqty. }
-        { apply* IHGamma. } }
+      introv Henv Hvar. unfolds vars.
+      forwards Hmem : Nth_mem Hvar.
+      forwards* [ Hmem' ? ] : mem_filter_inv Hmem.
+      forwards [ G1 (G2 & Heq) ] : mem_inv_middle Hmem' ; subst.
+      applys ok_type_lct.
+      applys* ok_env_type.
     Qed.
 
     Lemma ok_term_lct :
@@ -196,9 +303,13 @@ Module Soundness (P : PAT).
     Proof.
       introv ttype. induction* ttype.
       { Case "TmVar". apply* ok_env_lct. }
-      { Case "TmLam". constructor. with_hyp (ok_type _ _ _) as Htyp. applys ok_type_lct Htyp. auto. }
+      { Case "TmLam". constructor*. with_hyp (ok_type _ _ _) as Htyp. applys ok_type_lct Htyp. }
       { Case "TmApp". inverts* IHttype1. }
-      { Case "TmTyApp". inverts* IHttype. (* Lemma here *) }
+      { Case "TmTyApp".
+        inverts* IHttype.
+        rewrite ty_subst_open.
+        apply ty_defreshen_lc. apply* ty_lc_subst. apply ty_freshen_lc. apply* ok_type_lct. }
+    Qed.
 
     Lemma ok_term_lc :
       forall Gamma t ty,
@@ -206,153 +317,151 @@ Module Soundness (P : PAT).
         tm_lc t.
     Proof.
       introv ttype. induction* ttype.
-      { Case "TmLam". constructor*. admit. } Admitted.
+      { Case "TmLam". constructor*. applys* ok_type_lct. }
+      { Case "TmTyLam". constructor*. applys* ok_type_lct. }
+    Qed.
 
     Lemma ok_data_strengthen_var :
       forall G1 G2 ty' d,
-        ok_data (G1 ++ BindVar (Some ty') :: G2) d ->
-        ok_data (G1 ++ BindVar None :: G2) d.
+        ok_data (G1 ++ BindVar ty' :: G2) d ->
+        ok_data (G1 ++ SkipVar :: G2) d.
     Proof. Admitted.
 
     Lemma ok_kind_strengthen_var :
       forall G1 G2 ty' k,
-        ok_kind (G1 ++ BindVar (Some ty') :: G2) k ->
-        ok_kind (G1 ++ BindVar None :: G2) k.
+        ok_kind (G1 ++ BindVar ty' :: G2) k ->
+        ok_kind (G1 ++ SkipVar :: G2) k.
     Proof. Admitted.
 
     Lemma ok_type_strengthen_var :
       forall G1 G2 ty' ty k,
-        ok_type (G1 ++ BindVar (Some ty') :: G2) ty k ->
-        ok_type (G1 ++ BindVar None :: G2) ty k.
+        ok_type (G1 ++ BindVar ty' :: G2) ty k ->
+        ok_type (G1 ++ SkipVar :: G2) ty k.
     Proof. Admitted.
 
     Lemma ok_env_strengthen_var :
       forall G1 G2 ty,
-        ok_env (G1 ++ BindVar (Some ty) :: G2) ->
-        ok_env (G1 ++ BindVar None :: G2).
-    Proof.
-      introv Henv. induction* G1 ; rew_list in *. inverts* Henv.
-      destruct* a ; inverts* Henv. constructor*.
-      apply* ok_data_strengthen_var. apply* ok_type_strengthen_var. unfolds tnames. rew_listx in *.
-      unfold is_tname in *. rew_mcore* in *.
-      constructor. apply* IHG1. apply* ok_kind_strengthen_var.
-      constructor. apply* IHG1. apply* ok_type_strengthen_var.
-    Qed.
+        ok_env (G1 ++ BindVar ty :: G2) ->
+        ok_env (G1 ++ SkipVar :: G2).
+    Proof. Admitted.
+    (*   introv Henv. induction* G1 ; rew_list in *. inverts* Henv. *)
+    (*   destruct* a ; inverts* Henv. constructor*. *)
+    (*   apply* ok_data_strengthen_var. apply* ok_type_strengthen_var. unfolds tnames. rew_listx in *. *)
+    (*   unfold is_tname in *. rew_env* in *. *)
+    (*   constructor. apply* IHG1. apply* ok_kind_strengthen_var. *)
+    (*   constructor. apply* IHG1. apply* ok_type_strengthen_var. *)
+    (* Qed. *)
 
     Lemma ok_data_drop_var :
       forall G1 G2 d,
-        ok_data (G1 ++ BindVar None :: G2) d ->
+        ok_data (G1 ++ SkipVar :: G2) d ->
         ok_data (G1 ++ G2) d.
     Proof. Admitted.
 
     Lemma ok_kind_drop_var :
       forall G1 G2 k,
-        ok_kind (G1 ++ BindVar None :: G2) k ->
+        ok_kind (G1 ++ SkipVar :: G2) k ->
         ok_kind (G1 ++ G2) k.
     Proof. Admitted.
 
     Lemma ok_type_drop_var :
       forall G1 G2 ty k,
-        ok_type (G1 ++ BindVar None :: G2) ty k ->
+        ok_type (G1 ++ SkipVar :: G2) ty k ->
         ok_type (G1 ++ G2) ty k.
     Proof. Admitted.
 
     Lemma ok_env_drop_var :
       forall G1 G2,
-        ok_env (G1 ++ BindVar None :: G2) ->
+        ok_env (G1 ++ SkipVar :: G2) ->
         ok_env (G1 ++ G2).
-    Proof.
-      introv Henv. induction* G1 ; rew_list in *. inverts* Henv.
-      destruct* a ; inverts* Henv. constructor*.
-      apply* ok_data_drop_var. apply* ok_type_drop_var. unfolds tnames. rew_listx in *.
-      unfold is_tname in *. rew_mcore* in *.
-      constructor. apply* IHG1. apply* ok_kind_drop_var.
-      constructor. apply* IHG1. apply* ok_type_drop_var.
-    Qed.
+    Proof. Admitted.
+    (*   introv Henv. induction* G1 ; rew_list in *. inverts* Henv. *)
+    (*   destruct* a ; inverts* Henv. constructor*. *)
+    (*   apply* ok_data_drop_var. apply* ok_type_drop_var. unfolds tnames. rew_listx in *. *)
+    (*   unfold is_tname in *. rew_env* in *. *)
+    (*   constructor. apply* IHG1. apply* ok_kind_drop_var. *)
+    (*   constructor. apply* IHG1. apply* ok_type_drop_var. *)
+    (* Qed. *)
+
+    Lemma tm_freshen_preservation :
+      forall Gamma t ty b,
+        is_var b ->
+        ok_term Gamma t ty ->
+        ok_term (b :: Gamma) (tm_freshen t 0) ty.
+    Proof. Admitted.
+
+    Lemma tm_ty_freshen_preservation :
+      forall Gamma t ty b,
+        is_tvar b ->
+        ok_term Gamma t ty ->
+        ok_term (b :: Gamma) (tm_ty_freshen t 0) ty.
+    Proof. Admitted.
 
     Lemma ok_term_drop_var :
       forall G1 G2 t ty,
-        ok_term (G1 ++ BindVar None :: G2) t ty ->
+        ok_term (G1 ++ SkipVar :: G2) t ty ->
         ok_term (G1 ++ G2) (tm_defreshen t (length (vars G1))) ty.
     Proof.
       introv ttype.
-      remember (G1 ++ BindVar None :: G2) as Gamma eqn:HGamma.
+      remember (G1 ++ SkipVar :: G2) as Gamma eqn:HGamma.
       gen G1.
       induction ttype ; intros ; subst*.
-      { Case "TmFVar". with_hyp (var_in _ _ _) as Hvar. rew_mcore in Hvar. unfold var_in in Hvar.
+      { Case "TmFVar". with_hyp (var_in _ _ _) as Hvar. rew_env in Hvar. unfold var_in in Hvar.
         unfold tm_defreshen.
         lets [ in_vs1 | (m' & Heqm' & in_vs2') ] : Nth_app_inv Hvar.
-        { lets Hlt : Nth_inbound in_vs1. assert (Hnge : ~(x > length (vars G1))). apply* lt_gt_false.
-          rewrites (>> If_r Hnge). constructor. apply* ok_env_drop_var. unfold var_in. rew_mcore.
+        { lets Hlt : Nth_inbound in_vs1. simple_math.
+          constructor. apply* ok_env_drop_var. unfold var_in. rew_env.
           applys* Nth_app_l. }
         { lets [ (Heq0 & Heqty) | (m & Heqm & in_vs2) ] : Nth_cons_inv in_vs2' ; subst.
           { inverts Heqty. }
-          { rew_nat. assert (Hge : S (length (vars G1) + m) > length (vars G1)). nat_math.
-            rewrites (>> If_l Hge).
-            constructor. apply* ok_env_drop_var. unfold var_in. rew_mcore.
+          { simple_math. constructor. apply* ok_env_drop_var. unfold var_in. rew_env.
             applys_eq* (>> Nth_app_r in_vs2). nat_math. } } }
       { Case "TmLam". constructor. apply* ok_type_drop_var.
         rewrite tm_open_defreshen_comm.
-        applys_eq* (IHttype (BindVar (Some ty1) :: G1)). rew_mcore*. }
+        applys_eq* (IHttype (BindVar ty1 :: G1)). rew_env*. }
       { Case "TmTyLam". constructor. apply* ok_kind_drop_var.
         rewrite tm_ty_open_defreshen_comm.
-        applys_eq* (IHttype (BindTvar (Some k) :: G1)). rew_mcore*. }
+        applys_eq* (IHttype (BindTvar k :: G1)). rew_env*. }
       { Case "TmTyApp". constructors*. apply* ok_type_drop_var. }
     Qed.
 
-    Lemma tm_subst_preservation_gen :
+    Lemma tm_subst_preservation :
       forall G1 G2 t t' ty1 ty2,
-        ok_term (G1 ++ BindVar (Some ty1) :: G2) t ty2 ->
-        ok_term (G1 ++ BindVar None :: G2) t' ty1 ->
-        ok_term (G1 ++ BindVar None :: G2) (tm_subst t (length (vars G1)) t') ty2.
+        ok_term (G1 ++ BindVar ty1 :: G2) t ty2 ->
+        ok_term (G1 ++ SkipVar :: G2) t' ty1 ->
+        ok_term (G1 ++ SkipVar :: G2) (tm_subst t (length (vars G1)) t') ty2.
     Proof.
       introv ttype.
-      remember (G1 ++ BindVar (Some ty1) :: G2) as Gamma eqn:HGamma.
+      remember (G1 ++ BindVar ty1 :: G2) as Gamma eqn:HGamma.
       gen t' G1.
       induction ttype ; intros ; subst*.
       { Case "TmFVar".
-        with_hyp (var_in _ _ _) as Hvar. rew_mcore in Hvar. unfold var_in in Hvar.
+        with_hyp (var_in _ _ _) as Hvar. rew_env in Hvar. unfold var_in in Hvar.
         unfold tm_subst.
         lets [ in_vs1 | (m' & Heqm' & in_vs2') ] : Nth_app_inv Hvar.
-        { lets Hlt : Nth_inbound in_vs1. assert (Hneq : x <> length (vars G1)). nat_math.
-          rewrites (>> If_r Hneq). constructor. apply* ok_env_strengthen_var. unfold var_in. rew_mcore.
+        { lets Hlt : Nth_inbound in_vs1. simple_math.
+          constructor. apply* ok_env_strengthen_var. unfold var_in. rew_env.
           applys* Nth_app_l. }
         { lets [ (Heq0 & Heqty) | (m & Heqm & in_vs2) ] : Nth_cons_inv in_vs2'.
-          { inverts* Heqty. assert (Heq : x = length (vars G1)). nat_math.
-            rewrites* (>> If_l Heq). }
-          { assert (Hneq : x <> length (vars G1)). nat_math.
-            rewrites (>> If_r Hneq). constructor. apply* ok_env_strengthen_var. unfold var_in. rew_mcore.
-            applys_eq* (>> Nth_app_r (vars G1 ++ [BindVar None]) in_vs2) ; rew_list~. nat_math. } } }
+          { inverts* Heqty. simple_math. }
+          { simple_math. constructor. apply* ok_env_strengthen_var. unfold var_in. rew_env.
+            applys_eq* (>> Nth_app_r (vars G1 ++ [SkipVar]) in_vs2) ; rew_list~. nat_math. } } }
       { Case "TmLam". constructor. applys* ok_type_strengthen_var ty1.
         rewrite tm_open_subst_comm.
-        applys_eq* (IHttype (tm_freshen t' 0) (BindVar (Some ty0) :: G1)). rew_mcore*.
+        applys_eq* (IHttype (tm_freshen t' 0) (BindVar ty0 :: G1)). rew_env*.
         rew_list. applys* tm_freshen_preservation. applys* ok_term_lc. }
       { Case "TmTyLam". constructor. applys* ok_kind_strengthen_var ty1.
         rewrite tm_ty_open_subst_comm.
-        applys_eq* (IHttype (tm_ty_freshen t' 0) (BindTvar (Some k) :: G1)). rew_mcore*.
+        applys_eq* (IHttype (tm_ty_freshen t' 0) (BindTvar k :: G1)). rew_env*.
         rew_list. applys* tm_ty_freshen_preservation. applys* ok_term_lc. }
       { Case "TmTyApp". constructors*. applys* ok_type_strengthen_var ty1. }
     Qed.
 
     Lemma tm_ty_subst_preservation :
       forall Gamma t ty ty' k,
-        ok_term (BindTvar (Some k) :: Gamma) (tm_ty_open t) (ty_open ty) ->
+        ok_term (BindTvar k :: Gamma) (tm_ty_open t) (ty_open ty) ->
         ok_type Gamma ty' k ->
         ok_term Gamma (tm_ty_bsubst t 0 ty') (ty_bsubst ty 0 ty').
-    Proof. Admitted.
-
-    Lemma tm_subst_preservation :
-      forall Gamma t t' ty1 ty2,
-        ok_term (BindVar (Some ty1) :: Gamma) t ty2 ->
-        ok_term Gamma t' ty1 ->
-        ok_term Gamma (tm_defreshen (tm_subst t 0 (tm_freshen t' 0)) 0) ty2.
-    Proof. Admitted.
-
-    Lemma tm_bsubst_preservation :
-      forall Gamma t t' ty1 ty2,
-        ok_term (BindVar (Some ty1) :: Gamma) (tm_open t) ty2 ->
-        ok_term Gamma t' ty1 ->
-        ok_term Gamma (tm_bsubst t 0 t') ty2.
     Proof. Admitted.
 
     Theorem preservation :
@@ -366,7 +475,10 @@ Module Soundness (P : PAT).
       induction ttype ; intros ; inverts tstep
       ; try (with_hyp (is_context _) as ctx ; with_hyp (_ = _) as eq
              ; inverts ctx ; inverts* eq).
-      { Case "TmApp". inverts ttype1. applys* tm_bsubst_preservation. }
+      { Case "TmApp". inverts ttype1. rewrite tm_subst_open.
+        applys* ok_term_drop_var empty_env Gamma.
+        applys* tm_subst_preservation empty_env Gamma ty1.
+        applys* tm_freshen_preservation ttype2. }
       { Case "TmTyApp". inverts ttype. applys* tm_ty_subst_preservation. }
     Qed.
   End Soundness.
